opentheory/theories/word10/word10-word.ml
@@ -282,15 +282,8 @@ let word10_to_list_def = new_axiom
 
 new_constant ("list_to_word10", `:bool list -> word10`);;
 
-let list_to_word10_nil = new_axiom
-  `list_to_word10 [] = num_to_word10 0`
-and list_to_word10_cons = new_axiom
-  `!h t.
-     list_to_word10 (CONS h t) =
-     if h then word10_add (word10_shl (list_to_word10 t) 1) (num_to_word10 1)
-     else word10_shl (list_to_word10 t) 1`;;
-
-let list_to_word10_def = CONJ list_to_word10_nil list_to_word10_cons;;
+let list_to_word10_def = new_axiom
+  `!l. list_to_word10 l = num_to_word10 (bits_to_num l)`;;
 
 new_constant ("is_word10_list", `:bool list -> bool`);;
 
@@ -333,8 +326,14 @@ let length_word10_to_list = new_axiom
 let is_word10_to_list = new_axiom
   `!w. is_word10_list (word10_to_list w)`;;
 
-let bits_to_num_to_word10 = new_axiom
-   `!l. num_to_word10 (bits_to_num l) = list_to_word10 l`;;
+let list_to_word10_nil = new_axiom
+   `list_to_word10 [] = num_to_word10 0`;;
+
+let list_to_word10_cons = new_axiom
+   `!h t.
+      list_to_word10 (CONS h t) =
+      if h then word10_add (num_to_word10 1) (word10_shl (list_to_word10 t) 1)
+      else word10_shl (list_to_word10 t) 1`;;
 
 let word10_bit_div = new_axiom
   `!w n. word10_bit w n = ODD (word10_to_num w DIV (2 EXP n))`;;
@@ -345,13 +344,14 @@ let nil_to_word10_to_num = new_axiom
 let cons_to_word10_to_num = new_axiom
    `!h t.
       word10_to_num (list_to_word10 (CONS h t)) =
-      (2 * word10_to_num (list_to_word10 t) + (if h then 1 else 0)) MOD word10_size`;;
+      ((if h then 1 else 0) + 2 * word10_to_num (list_to_word10 t)) MOD
+      word10_size`;;
 
 let list_to_word10_to_num_bound = new_axiom
   `!l. word10_to_num (list_to_word10 l) < 2 EXP (LENGTH l)`;;
 
 let list_to_word10_to_num_bound_suc = new_axiom
-  `!l. 2 * word10_to_num (list_to_word10 l) + 1 < 2 EXP (SUC (LENGTH l))`;;
+  `!l. 1 + 2 * word10_to_num (list_to_word10 l) < 2 EXP (SUC (LENGTH l))`;;
 
 let cons_to_word10_to_num_bound = new_axiom
    `!h t.
@@ -424,7 +424,8 @@ let word10_shr_list = new_axiom
          else list_to_word10 (drop n (take word10_width l)))`;;
 
 let word10_eq_bits = new_axiom
-  `!w1 w2. (!i. i < word10_width ==> word10_bit w1 i = word10_bit w2 i) ==> w1 = w2`;;
+  `!w1 w2.
+     (!i. i < word10_width ==> word10_bit w1 i = word10_bit w2 i) ==> w1 = w2`;;
 
 let num_to_word10_cons = new_axiom
   `!n.
@@ -487,7 +488,7 @@ let list_to_word10_to_list_conv =
        take_conv);;
 
 let numeral_to_word10_list_conv =
-    let zero_conv = REWR_CONV (SYM (CONJUNCT1 list_to_word10_def)) in
+    let zero_conv = REWR_CONV (SYM list_to_word10_nil) in
     let numeral_conv = REWR_CONV (SYM (SPEC `NUMERAL n` num_to_word10_cons)) in
     let rec rewr_conv tm =
         (zero_conv ORELSEC
